prove wp_sim_imply_refine

coqimp/ext/finaltheorem.v
@@ -1,5 +1,5 @@
-(*+ Final Theorem Proof +*)
-Require Import Coqlib. 
+(*+ Final Theorem Proof +*)  
+Require Import Coqlib.     
 Require Import Maps.
 
 Require Import Classical_Prop.
@@ -27,6 +27,106 @@ Unset Strict Implicit.
 Open Scope code_scope.
 Open Scope mem_scope.
 
+(** Auxiliary Lemmas about multi-steps *)
+Inductive n_tau_step {prog : Type} (step : prog -> msg -> prog -> Prop) :
+  nat -> prog -> prog -> Prop :=
+| tau_step0 : forall p, n_tau_step step 0%nat p p
+| tau_step_Sn : forall (p p' p'' : prog) n, n_tau_step step n p p' -> step p' tau p'' ->
+                                             n_tau_step step (S n) p p''.
+
+Lemma Hstar_step_code_unchange :
+  forall C PrimSet HS HP',
+    star_tau_step HP__ (C, PrimSet, HS) HP' ->
+    exists HS', HP' = (C, PrimSet, HS').
+Proof.
+Admitted.
+
+Lemma Lstar_step_code_unchange :
+  forall C S LP',
+    star_tau_step LP__ (C, S) LP' ->
+    exists S', LP' = (C, S').
+Proof.
+Admitted.
+
+Lemma n_tau_step_front_back :
+  forall n A P P' P'' (step : A -> msg -> A -> Prop),
+    n_tau_step step n P P' -> step P' tau P'' ->
+    exists P0, step P tau P0 /\ n_tau_step step n P0 P''.
+Proof.
+  induction n; intros.
+  inv H.
+  exists P''; split; eauto.
+  econstructor; eauto.
+  inv H.
+  eapply IHn with (step := step) in H2; eauto.
+  destruct H2 as [P0 [Hstep H2] ].
+  exists P0; split; eauto.
+  econstructor; eauto.
+Qed.
+
+Lemma star_step_impl_n_step :
+  forall A P P' (step : A -> msg -> A -> Prop),
+    star_tau_step step P P' -> exists n, n_tau_step step n P P'.
+Proof.
+  intros.
+  induction H.
+  exists 0%nat; econstructor; eauto.
+  destruct IHstar_tau_step as [n IHstar_tau_step].
+  exists (S n); econstructor; eauto.
+Qed.
+
+Lemma n_step_impl_star_step :
+  forall n A P P' (step : A -> msg -> A -> Prop),
+    n_tau_step step n P P' -> star_tau_step step P P'.
+Proof.
+  induction n; intros.
+  inv H.
+  econstructor; eauto.
+  inv H.
+  eapply multi_tau_step; eauto.
+Qed.
+
+Lemma multi_tau_step_front_back :
+  forall A P P' P'' (step : A -> msg -> A -> Prop),
+    star_tau_step step P P' -> step P' tau P'' ->
+    exists P0, step P tau P0 /\ star_tau_step step P0 P''.
+Proof.
+  intros.
+  eapply star_step_impl_n_step in H.
+  destruct H as [n H].
+  eapply n_tau_step_front_back with (step := step) in H; eauto.
+  destruct H as (P0 & Hstep & Hn_tau_step).
+  exists P0; split; eauto.
+  eapply n_step_impl_star_step; eauto.
+Qed.
+
+Lemma n_tau_step_cons :
+  forall m n A P P' P'' (step : A -> msg -> A -> Prop),
+    n_tau_step step n P P' -> n_tau_step step m P' P'' ->
+    n_tau_step step (Nat.add n m) P P''.
+Proof.
+  induction m; intros.
+  inv H0.
+  rewrite Nat.add_0_r; eauto.
+  inv H0.
+  eapply IHm in H; eauto.
+  rewrite <- plus_n_Sm.
+  econstructor; eauto.
+Qed.
+
+Lemma multi_tau_step_cons :
+  forall A P P' P'' (step : A -> msg -> A -> Prop),
+    star_tau_step step P P' -> star_tau_step step P' P'' ->
+    star_tau_step step P P''.
+Proof.
+  intros.
+  generalize dependent P.
+  induction H0; intros; eauto.
+  eapply IHstar_tau_step in H1; eauto.
+  eapply multi_tau_step; eauto.
+Qed.
+
+(** final theorem proof *)
 CoInductive IdxEtrace {tprog} (step : tprog -> msg -> tprog -> Prop): Index -> tprog -> Etr -> Prop :=
 | IdxEtr_tau1 : forall P P' P'' idx idx',
     star_tau_step step P P' -> step P' tau P'' ->
@@ -40,119 +140,125 @@ CoInductive IdxEtrace {tprog} (step : tprog -> msg -> tprog -> Prop): Index -> t
     star_tau_step step P P' -> step P' (out v) P'' ->
     IdxEtrace step idx' P'' etr -> IdxEtrace step idx P (outEtr v etr).
 
-(*
-Inductive n_tau_step {prog : Type} (step : prog -> msg -> prog -> Prop) :
-  Index -> prog -> prog -> Prop :=
-| Zero_tau_step : forall p idx, ~ (exists idx', idx' ⩹ idx) -> n_tau_step step idx p p
-| Multi_tau_step : forall (p p' p'' p''': prog) idx_i idx_j,
-    star_tau_step step p p' -> step p' tau p'' -> idx_j ⩹ idx_i ->
-    n_tau_step step idx_j p'' p''' -> 
-    n_tau_step step idx_i p p'''.
-
-Lemma Etr_emp_n_step :
-  forall A (P : A) ndx (step : A -> msg -> A -> Prop),
-    Etrace step P empEtr -> well_founded LtIndex ->
-    exists P', n_tau_step step ndx P P'.
+Lemma n_tau_step_wp_preserve :
+  forall n LP LP' HP idx,
+    n_tau_step LP__ n LP LP' -> wp_sim idx LP HP ->
+    exists idx_j HP' m, n_tau_step HP__ m HP HP' /\ wp_sim idx_j LP' HP'.
 Proof.
-  intros.
-  generalize dependent P.
-  generalize dependent step.
-  unfold well_founded in H0.
-  specialize (H0 ndx).
-  induction H0; intros.
-  inv H1.
-  destruct x.
-  destruct n, n0.
+  induction n; intros.
+  inv H.
+  exists idx HP 0%nat.
+  split; eauto.
+  econstructor; eauto.
+  inv H.
+  lets Hn_tau_step : H2.
+  eapply n_tau_step_front_back with (step := LP__) in Hn_tau_step; eauto.
+  destruct Hn_tau_step as (P0 & HLP__ & Hn_tau_step).
+  inv H0.
+  clear H1 H4.
+  lets Hwp_sim_prop : HLP__.
+  eapply H in Hwp_sim_prop; eauto.
+  clear H.
+  destruct Hwp_sim_prop as [(idx1 & Hlt & Hwp_sim) | (idx1 & HP' & HP'' & HHstar_step & HHstep & Hwp_sim)].
   {
-    exists P.
-    eapply Zero_tau_step.
-    intro.
-    destruct H1.
-    inv H1; try omega.
+    eapply IHn in Hwp_sim; eauto.
   }
   {
-    eapply H0 in H4; eauto.
-    Focus 2.
-    instantiate (1 := (0%nat, n0)); econstructor; eauto.
-    destruct H4 as [P''' H4].
-    exists P'''.
-    eapply Multi_tau_step; eauto.
-    econstructor; eauto.
-  }
-  {
-    eapply H0 in H4; eauto.
-    Focus 2.
-    instantiate (1 := (n, 0%nat)); econstructor; eauto.
-    destruct H4 as [P''' H4].
-    exists P'''.
-    eapply Multi_tau_step; eauto.
-    econstructor; eauto.
-  }
-  {
-    eapply H0 in H4; eauto.
-    Focus 2.
-    instantiate (1 := (S n, n0)).
-    econstructor; eauto.
-    destruct H4 as [P''' H4].
-    exists P'''.
-    eapply Multi_tau_step; eauto.
+    eapply IHn in Hwp_sim; eauto.
+    destruct Hwp_sim as (idx_j & HP0 & m & HH_n_steps & Hwp_sim).
+    eapply star_step_impl_n_step in HHstar_step.
+    destruct HHstar_step as (n' & HHstar_step).
+    exists idx_j HP0 (Nat.add (S n') m).
+    split; eauto.
+    eapply n_tau_step_cons; eauto.
     econstructor; eauto.
   }
 Qed.
 
-Lemma LEtr_emp_n_step_H_progress :
-  forall LP LP' HP ndx idx,
-    well_founded LtIndex ->
-    n_tau_step LP__ ndx LP LP' -> wp_sim idx LP HP -> idx ⩹ ndx ->
-    (exists HP' HP'', star_step HP__ HP HP' /\ HP__ HP' tau HP'').
+Lemma star_tau_step_wp_preserve :
+  forall LP LP' HP idx,
+    star_tau_step LP__ LP LP' -> wp_sim idx LP HP ->
+    exists idx_j HP', star_tau_step HP__ HP HP' /\ wp_sim idx_j LP' HP'.
 Proof.
   intros.
-  generalize dependent LP.
-  generalize dependent LP'.
-  generalize dependent HP.
-  generalize dependent idx.
-  unfold well_founded in H. 
-  specialize (H ndx).
-  induction H; intros.
-  inv H1.
-  contradiction H4; eauto.
-  inv H3.
-  clear H8 H9.
-  inv H4.
-  {
-    eapply H1 in H5.
-    clear H1.
-    destruct H5.
-    {
-      destruct H1 as [idx1 [Hlt Hwp_sim] ].
-      eapply H0 in Hwp_sim.
-      eauto.
-      instantiate(1 := idx); eauto.
-      eauto.
-      
-    }
-  }
-  
-  generalize dependent HP.
-  generalize dependent idx.
-  induction H; intros.
-  contradiction H; eauto.
-  inv H4. 
-  clear H6 H7.
-  
-  
-  induction H1; intros.
-  {
-    inv H0.
-    false.
-    contradiction H2.
-    exists (n, m').
-    econstructor; eauto.
-    Print Index.
-  }
- *)
+  eapply star_step_impl_n_step in H.
+  destruct H.
+  eapply n_tau_step_wp_preserve in H; eauto.
+  destruct H as (idx_j & HP' & m & Hn_tau_step & Hwp_sim).
+  eapply n_step_impl_star_step in Hn_tau_step; eauto.
+Qed.
 
-Lemma wp_sim_ensures_refinement' :
+Lemma wp_sim_ensures_refinement_empEtr :
+  forall C Cas S pc npc PrimSet HS idx,
+    C ⊥ Cas -> wp_sim idx (C ⊎ Cas, (S, pc, npc)) (C, PrimSet, HS) ->
+    Etrace LP__ (C ⊎ Cas, (S, pc, npc)) empEtr ->
+    IdxEtrace HP__ idx (C, PrimSet, HS) empEtr.
+Proof.
+  cofix Hp; intros.
+  inv H1.
+  lets Hstar_step : H2.
+  eapply multi_tau_step_front_back with (step := LP__) in Hstar_step; eauto.
+  destruct Hstar_step as (P0 & Hstep & Hstar).
+  inv H0.
+  clear H5 H6.
+  lets Hwp_prop : Hstep.
+  eapply H1 in Hwp_prop; eauto.
+  clear H1; destruct Hwp_prop as [(idx1 & Hlt & Hwp_sim) | (idx1 & HP' & HP'' & Hstar_step & HHstep & Hwp_sim)].
+  {
+    inv Hstep.
+    eapply IdxEtr_tau2; eauto.
+    instantiate (1 := (C, PrimSet, HS)); econstructor; eauto.
+    eapply Hp; eauto.
+    clear - H4 Hstar.
+    inv H4.
+    eapply multi_tau_step_cons in H; eauto.
+    eapply Etr_tau; eauto.
+  }
+  {
+    inv Hstep.
+    eapply IdxEtr_tau1; eauto.
+    instantiate (1 := idx1).
+    eapply Hstar_step_code_unchange in Hstar_step; eauto.
+    destruct Hstar_step as [HS' Hstar_step]; subst.
+    inv HHstep.
+    eapply Hp; eauto.
+    clear - Hstar H4.
+    inv H4.
+    eapply multi_tau_step_cons in H; eauto.
+    eapply Etr_tau; eauto.
+    eapply Hp; eauto.    
+    clear - Hstar H4.
+    inv H4.
+    eapply multi_tau_step_cons in H; eauto.
+    eapply Etr_tau; eauto.
+  }
+Qed.
+
+Lemma wp_sim_ensures_refinement_abort :
+  forall  C Cas S pc npc PrimSet HS idx,
+    C ⊥ Cas -> wp_sim idx (C ⊎ Cas, (S, pc, npc)) (C, PrimSet, HS) ->
+    Etrace LP__ (C ⊎ Cas, (S, pc, npc)) abortEtr ->
+    IdxEtrace HP__ idx (C, PrimSet, HS) abortEtr.
+Proof.
+  intros.
+  inv H1.
+  eapply star_tau_step_wp_preserve in H2; eauto.
+  destruct H2 as (idx_j & HP' & HHstar_step & Hwp_sim).
+  clear H0.
+  inv Hwp_sim.
+  clear H0 H1.
+  eapply H2 in H3.
+  clear H2.
+  destruct H3 as (HP'0 & Hstar & Habort). 
+  assert (Ht : star_tau_step HP__ (C, PrimSet, HS) HP'0).
+  eapply multi_tau_step_cons with (P' := HP'); eauto.
+  clear HHstar_step Hstar.
+  econstructor; eauto.
+  Unshelve.
+  exact tau.
+Qed.
+
+Lemma wp_sim_ensures_idx_refinement :
   forall C Cas S pc npc PrimSet HS B idx,
     C ⊥ Cas -> wp_sim idx (C ⊎ Cas, (S, pc, npc)) (C, PrimSet, HS) ->
     Etrace LP__ (C ⊎ Cas, (S, pc, npc)) B ->
@@ -161,24 +267,87 @@ Proof.
   cofix Hp; intros.
   destruct B.
   {
-    inv H1.
+    eapply wp_sim_ensures_refinement_empEtr; eauto.
+  }
+  {
+    eapply wp_sim_ensures_refinement_abort; eauto.
+  }
+  {
+    inv H1. 
+    eapply star_tau_step_wp_preserve in H0; eauto.
+    destruct H0 as (idx_j & HP' & HHstar & Hwp_sim).
+    inv Hwp_sim.
+    clear H0 H2.
+    lets Hwp_sim_prop : H6.
+    eapply H1 in Hwp_sim_prop; eauto.
+    clear H1.
+    destruct Hwp_sim_prop as (idx1 & HP'0 & HP'' & HHstar_step & HHstep & Hwp_sim).
+    econstructor.
+    instantiate (1 := HP'0).
+    eapply multi_tau_step_cons; eauto.
+    eauto.
+    instantiate (1 := idx1).
+    eapply Hstar_step_code_unchange in HHstar; eauto.
+    destruct HHstar as (HS' & HHstar); subst.
+    eapply Hstar_step_code_unchange in HHstar_step; eauto.
+    destruct HHstar_step as (HS'' & HHstar_step); subst.
+    inv HHstep.
+    eapply Lstar_step_code_unchange in H4.
+    destruct H4 as [S' LP']; subst.
+    inv H6.
+    eapply Hp; eauto.
+  }
+Qed.
+
+Lemma IdxEtrace_impl_progress :
+  forall A idx (step : A -> msg -> A -> Prop) P,
+    IdxEtrace step idx P empEtr -> well_founded LtIndex ->
+    exists P' P'' idx', star_tau_step step P P' /\ step P' tau P'' /\ IdxEtrace step idx' P'' empEtr.
+Proof.
+  intros.
+  unfold well_founded in H0.
+  specialize (H0 idx).
+  generalize dependent P.
+  induction H0; intros.
+  inv H1.
+  {
+    exists P' P'' idx'.
+    repeat (split; eauto).
+  }
+  {
     inv H2.
     {
-      inv H0. 
-      clear H2 H5.
-      lets Hlp_step : H3.
-      eapply H1 in H3; eauto.
-      clear H1.
-      destruct H3 as [ [idx1 [Hlt H3] ] | [idx1 [ HP' [HP'' [Hstar [HPstep Hwpsim] ] ] ] ] ].
-      {
-        eapply IdxEtr_tau2.
-        instantiate (1 := (C, PrimSet, HS)).
-        eapply zero_tau_step; eauto.
-        eauto.
-        eapply Hp; eauto.
-      }
+      eapply H0; eauto.
+    }
+    {
+      exists p' P' idx'; eauto.
     }
   }
+Qed.
+
+Lemma IdxEtrace_imply_Etrace :
+  forall A (step : A -> msg -> A -> Prop) idx P B,
+    IdxEtrace step idx P B ->
+    Etrace step P B.
+Proof.
+  cofix Hp; intros.
+  destruct B.
+  {
+    (* tau *)
+    eapply IdxEtrace_impl_progress in H; eauto.
+    destruct H as (P' & P'' & idx' & Hstar_step & Hstep & HIdxEtrace).
+    econstructor; eauto.
+    eapply well_founded_LtIndex; eauto.
+  }
+  {
+    inv H.
+    econstructor; eauto.
+  }
+  {
+    inv H.
+    econstructor; eauto.
+  }
+Qed.
 
 Lemma wp_sim_ensures_refinement' :
   forall C Cas S pc npc PrimSet HS B idx,
@@ -186,11 +355,10 @@ Lemma wp_sim_ensures_refinement' :
     Etrace LP__ (C ⊎ Cas, (S, pc, npc)) B ->
     Etrace HP__ (C, PrimSet, HS) B.
 Proof.
-  cofix Hp.
   intros.
-  destruct B.
-  {
-  }
+  eapply wp_sim_ensures_idx_refinement in H1; eauto.
+  eapply IdxEtrace_imply_Etrace; eauto.
+Qed.
   
 (* Whole program simulation ensures refinement *)
 Lemma wp_sim_ensures_refinement :
